src/new_goose_lang/lib/typed_mem/typed_mem.v
@@ -3,11 +3,535 @@ From iris.proofmode Require Import tactics.
 From iris.proofmode Require Import environments.
 From Perennial.program_logic Require Import weakestpre.
 From Perennial.goose_lang Require Import proofmode.
-From Perennial.new_goose_lang.lib Require Export typed_mem.impl.
+From Perennial.new_goose_lang Require Export typed_mem.impl struct.impl slice.
 
 Set Default Proof Using "Type".
 
-Section go_lang.
+Section goose_lang.
   Context `{ffi_sem: ffi_semantics} `{!ffi_interp ffi} `{!heapGS Σ}.
   Context {ext_ty: ext_types ext}.
-End go_lang.
+
+  Inductive has_go_type: val → go_type → Prop :=
+  | has_go_type_bool (b : bool) : has_go_type #b boolT
+
+  | has_go_type_uint64 (x : w64) : has_go_type #x uint64T
+  | has_go_type_uint32 (x : w32) : has_go_type #x uint32T
+  (* | has_go_type_uint16 (x : w16) : has_go_type #x uint16T *)
+  | has_go_type_uint8 (x : w8) : has_go_type #x uint8T
+  | has_go_type_int64 (x : w64) : has_go_type #x int64T
+  | has_go_type_int32 (x : w32) : has_go_type #x int32T
+  (* | has_go_type_int16 (x : w16) : has_go_type #x int16T *)
+  | has_go_type_int8 (x : w8) : has_go_type #x int8T
+
+  | has_go_type_string (x : string) : has_go_type #(str x) stringT
+  | has_go_type_slice (elem : go_type) (s : slice.t) : has_go_type (slice_val s) (sliceT elem)
+
+  (* FIXME: this does not require the vals to be well typed, which causes problems. *)
+  | has_go_type_struct (d : descriptor) (fs : list (string * val)) (H : Forall (λ x, True) fs)
+    : has_go_type (struct.mk_f d fs) (structT d)
+
+  | has_go_type_ptr (x : loc) : has_go_type #x ptrT
+  | has_go_type_ptr_nil : has_go_type nil ptrT
+
+  | has_go_type_func f x e : has_go_type (RecV f x e) funcT
+  | has_go_type_func_nil : has_go_type nil funcT
+
+  (* FIXME: interface typing *)
+
+  | has_go_type_map (key elem : go_type) (l : loc) : has_go_type #l (mapT key elem)
+  | has_go_type_map_nil key elem : has_go_type nil (mapT key elem)
+
+  | has_go_type_chan elem (l : loc) : has_go_type #l (chanT elem)
+  | has_go_type_chan_nil elem : has_go_type nil (chanT elem)
+  .
+
+  (*
+  Inductive has_go_abstract_type : val → go_abstract_type → Prop :=
+  | has_go_abstract_type_bool (b : bool) : has_go_abstract_type #b cellT
+
+  | has_go_abstract_type_uint64 (x : w64) : has_go_abstract_type #x cellT
+  | has_go_abstract_type_uint32 (x : w32) : has_go_abstract_type #x cellT
+  (* | has_go_abstract_type_uint16 (x : w16) : has_go_abstract_type #x uint16T *)
+  | has_go_abstract_type_uint8 (x : w8) : has_go_abstract_type #x cellT
+  | has_go_abstract_type_int64 (x : w64) : has_go_abstract_type #x cellT
+  | has_go_abstract_type_int32 (x : w32) : has_go_abstract_type #x cellT
+  (* | has_go_abstract_type_int16 (x : w16) : has_go_abstract_type #x int16T *)
+  | has_go_abstract_type_int8 (x : w8) : has_go_abstract_type #x cellT
+
+  | has_go_abstract_type_string (x : string) : has_go_abstract_type #(str x) cellT
+  | has_go_abstract_type_slice (elem : go_type) (s : slice.t) : has_go_abstract_type (slice_val s) prodT cellT $ prodT cellT $ prodT cellT unitT
+  | has_go_abstract_type_struct (d : descriptor) (fs : list (string * val)) : has_go_abstract_type (struct.mk_f d fs) (structT d)
+
+  | has_go_abstract_type_ptr (x : loc) : has_go_abstract_type #x ptrT
+  | has_go_abstract_type_ptr_nil : has_go_abstract_type nil ptrT
+
+  | has_go_abstract_type_func f x e : has_go_abstract_type (RecV f x e) funcT
+  | has_go_abstract_type_func_nil : has_go_abstract_type nil funcT
+
+  (* FIXME: interface typing *)
+
+  | has_go_abstract_type_map (key elem : go_type) (l : loc) : has_go_abstract_type #l (mapT key elem)
+  | has_go_abstract_type_map_nil key elem : has_go_abstract_type nil (mapT key elem)
+
+  | has_go_abstract_type_chan elem (l : loc) : has_go_abstract_type #l (chanT elem)
+  | has_go_abstract_type_chan_nil elem : has_go_abstract_type nil (chanT elem)
+  . *)
+
+  Ltac invc H := inversion H; subst; clear H.
+
+  Ltac inv_ty :=
+    repeat match goal with
+           | [ H: has_go_type _ ?t |- _ ] =>
+             first [ is_var t; fail 1 | invc H ]
+           end.
+
+  Theorem ty_size_offset t l j :
+    l +ₗ (length (flatten_ty t) + j)%nat = l +ₗ ty_size t +ₗ j.
+  Proof.
+    rewrite loc_add_assoc.
+    f_equal.
+    rewrite <- ty_size_length.
+    pose proof (ty_size_ge_0 t).
+    lia.
+  Qed.
+
+  Definition typed_pointsto_def l (dq : dfrac) (t : go_type) (v : val): iProp Σ :=
+    (([∗ list] j↦vj ∈ flatten_struct v, (l +ₗ j) ↦{dq} vj) ∗ ⌜ has_go_type v t ⌝)%I.
+  Definition typed_pointsto_aux : seal (@typed_pointsto_def). Proof. by eexists. Qed.
+  Definition typed_pointsto := typed_pointsto_aux.(unseal).
+  Definition typed_pointsto_eq : @typed_pointsto = @typed_pointsto_def := typed_pointsto_aux.(seal_eq).
+
+  Notation "l ↦[ t ] dq v" := (typed_pointsto l dq t v%V)
+                                   (at level 20, dq custom dfrac at level 1, t at level 50,
+                                    format "l  ↦[ t ] dq  v") : bi_scope.
+
+  Ltac unseal := rewrite ?typed_pointsto_eq /typed_pointsto_def.
+
+  Global Instance typed_pointsto_timeless l t q v: Timeless (l ↦[t]{q} v).
+  Proof. unseal. apply _. Qed.
+
+  Global Instance typed_pointsto_fractional l t v: fractional.Fractional (λ q, l ↦[t]{#q} v)%I.
+  Proof. unseal. apply _. Qed.
+
+  (*
+  Theorem typed_pointsto_singleton l q t v v0 :
+    flatten_struct v = [v0] ->
+    l ↦[t]{q} v ⊢@{_} l ↦{q} v0.
+  Proof.
+    intros Hv.
+    unseal.
+    rewrite Hv /=.
+    by rewrite loc_add_0 right_id.
+  Qed. *)
+
+  Theorem typed_pointsto_ty q l v t :
+    l ↦[t]{q} v ⊢@{_} ⌜has_go_type v t⌝.
+  Proof. unseal. iIntros "[_ %] !%//". Qed.
+
+  Theorem has_go_type_len v t :
+    has_go_type v t ->
+    length (flatten_struct v) = Z.to_nat (go_type_size t).
+  Proof.
+    unfold go_type_size.
+    induction 1; simpl; auto.
+    induction d.
+    + done.
+    + simpl. destruct a. simpl. admit.
+      (* FIXME: don't know that the fields of the struct have a typed *)
+  Qed.
+
+  Theorem typed_pointsto_frac_valid l q t v :
+    0 < go_type_size t →
+    l ↦[t]{#q} v -∗ ⌜(q ≤ 1)%Qp⌝.
+  Proof.
+    unseal.
+    iIntros (?) "[Hvals %Hhas_go_type]".
+    apply has_go_type_len in Hhas_go_type.
+    destruct (flatten_struct v); simpl in *.
+    - lia.
+    - iDestruct "Hvals" as "[Hl _]".
+      iDestruct (heap_pointsto_frac_valid with "Hl") as %Hq.
+      auto.
+  Qed.
+
+  Local Lemma typed_pointsto_agree_flatten l t q1 v1 q2 v2 :
+    length (flatten_struct v1) = length (flatten_struct v2) ->
+    l ↦[t]{q1} v1 -∗ l ↦[t]{q2} v2 -∗
+    ⌜flatten_struct v1 = flatten_struct v2⌝.
+  Proof.
+    unseal.
+    iIntros (Hlen) "[Hl1 _] [Hl2 _]".
+    generalize dependent (flatten_struct v1); intros l1.
+    generalize dependent (flatten_struct v2); intros l2.
+    clear.
+    iIntros (Hlen).
+    (iInduction l1 as [|v1 l1] "IH" forall (l l2 Hlen)).
+    { simpl in Hlen.
+      destruct l2; simpl in Hlen; try congruence.
+      auto. }
+    destruct l2; simpl in Hlen; try congruence.
+    simpl.
+    iDestruct "Hl1" as "[Hx1 Hl1]".
+    iDestruct "Hl2" as "[Hx2 Hl2]".
+    iDestruct (heap_pointsto_agree with "[$Hx1 $Hx2]") as "->".
+    setoid_rewrite loc_add_Sn.
+    iDestruct ("IH" $! (l +ₗ 1) l2 with "[] Hl1 Hl2") as %->; auto.
+  Qed.
+
+  Theorem typed_pointsto_agree l t q1 v1 q2 v2 :
+    l ↦[t]{q1} v1 -∗ l ↦[t]{q2} v2 -∗
+    ⌜v1 = v2⌝.
+  Proof.
+    iIntros "Hl1 Hl2".
+    iDestruct (typed_pointsto_ty with "Hl1") as %Hty1.
+    iDestruct (typed_pointsto_ty with "Hl2") as %Hty2.
+    pose proof (has_go_type_len Hty1).
+    pose proof (has_go_type_len Hty2).
+    iDestruct (typed_pointsto_agree_flatten with "Hl1 Hl2") as %Heq.
+    { congruence. }
+    iPureIntro.
+    eapply flatten_struct_inj; eauto.
+  Qed.
+
+  Global Instance typed_pointsto_persistent l t v : Persistent (l ↦[t]□ v).
+  Proof. rewrite typed_pointsto_eq. apply _. Qed.
+
+  Lemma typed_pointsto_persist l dq t v:
+    l ↦[t]{dq} v ==∗ l ↦[t]□ v.
+  Proof.
+    rewrite typed_pointsto_eq /typed_pointsto_def.
+    iIntros "[Ha %Ht]".
+    iDestruct (big_sepL_mono with "Ha") as "Ha".
+    2: iMod (big_sepL_bupd with "Ha") as "Ha".
+    { iIntros (???) "H".
+      iMod (heap_pointsto_persist with "H") as "H". iModIntro. iExact "H". }
+    iModIntro. iFrame "Ha". done.
+  Qed.
+
+  Lemma byte_pointsto_untype l q (x: u8) :
+    l ↦[byteT]{q} #x ⊣⊢ l ↦{q} #x.
+  Proof.
+    rewrite typed_pointsto_eq /typed_pointsto_def /=.
+    rewrite loc_add_0 right_id.
+    iSplit.
+    - iDestruct 1 as "[$ _]".
+    - iDestruct 1 as "$".
+      auto.
+  Qed.
+
+  Theorem base_pointsto_untype {l bt q v} :
+    match bt with
+    | unitBT => false
+    | _ => true
+    end = true ->
+    l ↦[baseT bt]{q} v ⊣⊢ l ↦{q} v ∗ ⌜has_go_type v (baseT bt)⌝.
+  Proof.
+    intros Hnotunit.
+    iSplit.
+    - iIntros "Hl".
+      iDestruct (typed_pointsto_ty with "Hl") as %Hty.
+      rewrite typed_pointsto_singleton; eauto.
+      inv_ty; simpl; auto.
+      congruence.
+    - iIntros "[Hl %]".
+      unseal.
+      iSplitL; auto.
+      inv_ty; simpl; try rewrite loc_add_0 right_id; auto.
+  Qed.
+
+  Theorem base_load_ty {bt} :
+    match bt with
+    | unitBT => false
+    | _ => true
+    end = true ->
+    load_ty (baseT bt) = (λ: "l", !(Var "l"))%V.
+  Proof.
+    destruct bt; simpl; intros; auto.
+    congruence.
+  Qed.
+
+  Theorem nat_scaled_offset_to_Z {v t} {i: nat} :
+    has_go_type v t ->
+    Z.of_nat (length (flatten_struct v)) * i =
+    ty_size t * Z.of_nat i.
+  Proof.
+    intros Hty.
+    rewrite (has_go_type_len Hty).
+    pose proof (ty_size_ge_0 t).
+    rewrite Z2Nat.id; auto.
+  Qed.
+
+  (* this is the core reasoning, not intended for external use *)
+  Local Theorem wp_AllocAt t stk E v :
+    has_go_type v t ->
+    {{{ True }}}
+      ref v @ stk; E
+    {{{ l, RET #l; l ↦[t] v }}}.
+  Proof.
+    iIntros (Hty Φ) "_ HΦ".
+    wp_apply wp_allocN_seq; first by word.
+    change (uint.nat 1) with 1%nat; simpl.
+    iIntros (l) "[Hl _]".
+    iApply "HΦ".
+    unseal.
+    iSplitL; auto.
+    rewrite Z.mul_0_r loc_add_0.
+    iFrame.
+  Qed.
+
+  Theorem wp_ref_to t stk E v :
+    has_go_type v t ->
+    {{{ True }}}
+      ref_to t v @ stk; E
+    {{{ l, RET #l; l ↦[t] v }}}.
+  Proof.
+    iIntros (Hty Φ) "_ HΦ".
+    wp_call.
+    wp_apply (wp_AllocAt t); auto.
+  Qed.
+
+  (* TODO: this is only because Goose doesn't use ref_zero *)
+  Theorem wp_ref_of_zero stk E t :
+    has_zero t ->
+    {{{ True }}}
+      ref (zero_val t) @ stk; E
+    {{{ l, RET #l; l ↦[t] (zero_val t) }}}.
+  Proof.
+    iIntros (Hzero Φ) "_ HΦ".
+    wp_apply (wp_AllocAt t); eauto.
+  Qed.
+
+  Theorem wp_ref_zero stk E t :
+    has_zero t ->
+    {{{ True }}}
+      ref_zero t #() @ stk; E
+    {{{ l, RET #l; l ↦[t] (zero_val t) }}}.
+  Proof.
+    iIntros (Hzero Φ) "_ HΦ".
+    wp_call.
+    wp_apply wp_ref_of_zero; eauto.
+  Qed.
+
+  Theorem wp_LoadAt stk E q l t v :
+    {{{ ▷ l ↦[t]{q} v }}}
+      load_ty t #l @ stk; E
+    {{{ RET v; l ↦[t]{q} v }}}.
+  Proof.
+    iIntros (Φ) ">Hl HΦ".
+    unseal.
+    iDestruct "Hl" as "[Hl %]".
+    hnf in H.
+    iAssert (▷ (([∗ list] j↦vj ∈ flatten_struct v, (l +ₗ j)↦{q} vj) -∗ Φ v))%I with "[HΦ]" as "HΦ".
+    { iIntros "!> HPost".
+      iApply "HΦ".
+      iSplit; eauto. }
+    (* TODO: we have to rename this so it doesn't conflict with a name generated
+  by induction; seems like a bug *)
+    rename l into l'.
+    (iInduction H as [ | | | | | | | | ] "IH" forall (l' Φ));
+      simpl;
+      wp_pures;
+      rewrite ?loc_add_0 ?right_id.
+    - inversion H; subst; simpl;
+        rewrite ?loc_add_0 ?right_id;
+        try wp_apply (wp_load with "[$]"); auto.
+      wp_pures.
+      iApply ("HΦ" with "[//]").
+    - rewrite big_opL_app.
+      iDestruct "Hl" as "[Hv1 Hv2]".
+      wp_apply ("IH" with "Hv1"); iIntros "Hv1".
+      wp_apply ("IH1" with "[Hv2]"); [ | iIntros "Hv2" ].
+      { erewrite has_go_type_flatten_length; eauto.
+        setoid_rewrite ty_size_offset.
+        rewrite Z.mul_1_r.
+        iFrame. }
+      wp_pures.
+      iApply "HΦ"; iFrame.
+      erewrite has_go_type_flatten_length by eauto.
+      setoid_rewrite ty_size_offset.
+      rewrite Z.mul_1_r.
+      by iFrame.
+    - wp_apply (wp_load with "[$]"); auto.
+    - wp_apply (wp_load with "[$]"); auto.
+    - wp_apply (wp_load with "[$]"); auto.
+    - wp_apply (wp_load with "[$]"); auto.
+    - wp_apply (wp_load with "[$]"); auto.
+    - wp_apply (wp_load with "[$]"); auto.
+    - wp_apply (wp_load with "[$]"); auto.
+  Qed.
+
+  Lemma tac_wp_load_ty Δ Δ' s E i K l q t v Φ :
+    MaybeIntoLaterNEnvs 1 Δ Δ' →
+    envs_lookup i Δ' = Some (false, typed_pointsto l q t v)%I →
+    envs_entails Δ' (WP fill K (Val v) @ s; E {{ Φ }}) →
+    envs_entails Δ (WP fill K (load_ty t (LitV l)) @ s; E {{ Φ }}).
+  Proof.
+    rewrite envs_entails_unseal=> ???.
+    rewrite -wp_bind. eapply bi.wand_apply; first by apply bi.wand_entails, wp_LoadAt.
+    rewrite into_laterN_env_sound -bi.later_sep envs_lookup_split //; simpl.
+    by apply bi.later_mono, bi.sep_mono_r, bi.wand_mono.
+  Qed.
+
+  Lemma tac_wp_load_ty_persistent Δ s E i K l t v Φ :
+    envs_lookup i Δ = Some (true, typed_pointsto l DfracDiscarded t v)%I →
+    envs_entails Δ (WP fill K (Val v) @ s; E {{ Φ }}) →
+    envs_entails Δ (WP fill K (load_ty t (LitV l)) @ s; E {{ Φ }}).
+  Proof.
+    rewrite envs_entails_unseal=> ? HΦ.
+    rewrite -wp_bind. eapply bi.wand_apply; first by apply bi.wand_entails, wp_LoadAt.
+    rewrite envs_lookup_split //; simpl.
+    iIntros "[#Hp Henvs]".
+    iSplitR; auto.
+    iIntros "!> _".
+    iApply HΦ.
+    iApply ("Henvs" with "Hp").
+  Qed.
+
+  Theorem wp_store stk E l v v' :
+    {{{ ▷ l ↦ v' }}} Store (Val $ LitV (LitLoc l)) (Val v) @ stk; E
+    {{{ RET LitV LitUnit; l ↦ v }}}.
+  Proof.
+    iIntros (Φ) "Hl HΦ". rewrite /Store.
+    wp_apply (wp_prepare_write with "Hl"); iIntros "[Hl Hl']".
+    by wp_apply (wp_finish_store with "[$Hl $Hl']").
+  Qed.
+
+  Theorem wp_StoreAt stk E l t v0 v :
+    has_go_type v t ->
+    {{{ ▷ l ↦[t] v0 }}}
+      (#l <-[t] v)%V @ stk; E
+    {{{ RET #(); l ↦[t] v }}}.
+  Proof.
+    intros Hty.
+    unseal.
+    iIntros (Φ) ">[Hl %] HΦ".
+    iAssert (▷ (([∗ list] j↦vj ∈ flatten_struct v, (l +ₗ j)↦ vj) -∗ Φ #()))%I with "[HΦ]" as "HΦ".
+    { iIntros "!> HPost".
+      iApply "HΦ".
+      iSplit; eauto. }
+    rename v into v'.
+    rename l into l'.
+    (iInduction H as [ | | | | | | | | ] "IH" forall (v' Hty l' Φ));
+      simpl;
+      rewrite ?loc_add_0 ?right_id;
+      wp_pures.
+    - invc Hty; invc H;
+        try match goal with
+            | [ H: lit_ty _ _ |- _ ] => invc H
+            end;
+        simpl;
+        rewrite ?loc_add_0 ?right_id;
+        try (wp_apply (wp_store with "[$]"); auto).
+      wp_pures.
+      iApply ("HΦ" with "[//]").
+    - rewrite big_opL_app.
+      erewrite has_go_type_flatten_length by eauto.
+      setoid_rewrite ty_size_offset.
+      invc Hty.
+      { by invc H1. (* can't be a pair and a base literal *) }
+      iDestruct "Hl" as "[Hv1 Hv2]".
+      wp_pures.
+      wp_apply ("IH" with "[//] Hv1").
+      iIntros "Hv1".
+      wp_pures.
+      rewrite Z.mul_1_r.
+      wp_apply ("IH1" with "[//] Hv2").
+      iIntros "Hv2".
+      iApply "HΦ".
+      simpl.
+      rewrite big_opL_app.
+      iFrame.
+      erewrite has_go_type_flatten_length by eauto.
+      setoid_rewrite ty_size_offset.
+      iFrame.
+    - inv_ty;
+        rewrite /= ?loc_add_0 ?right_id;
+        wp_apply (wp_store with "[$]"); auto.
+    - inv_ty;
+        rewrite /= ?loc_add_0 ?right_id;
+        wp_apply (wp_store with "[$]"); auto.
+    - invc Hty;
+        try match goal with
+            | [ H: lit_ty _ _ |- _ ] => invc H
+            end;
+        rewrite /= ?loc_add_0 ?right_id;
+        wp_apply (wp_store with "[$]"); auto.
+    - invc Hty;
+        try match goal with
+            | [ H: lit_ty _ _ |- _ ] => invc H
+            end;
+        rewrite /= ?loc_add_0 ?right_id;
+        wp_apply (wp_store with "[$]"); auto.
+    - invc Hty;
+        try match goal with
+            | [ H: lit_ty _ _ |- _ ] => invc H
+            end;
+        rewrite /= ?loc_add_0 ?right_id;
+        wp_apply (wp_store with "[$]"); auto.
+    - inv_ty;
+        rewrite /= ?loc_add_0 ?right_id;
+        wp_apply (wp_store with "[$]"); auto.
+    - inv_ty;
+        rewrite /= ?loc_add_0 ?right_id;
+        wp_apply (wp_store with "[$]"); auto.
+  Qed.
+
+  Lemma tac_wp_store_ty Δ Δ' Δ'' stk E i K l t v v' Φ :
+    has_go_type v' t ->
+    MaybeIntoLaterNEnvs 1 Δ Δ' →
+    envs_lookup i Δ' = Some (false, l ↦[t] v)%I →
+    envs_simple_replace i false (Esnoc Enil i (l ↦[t] v')) Δ' = Some Δ'' →
+    envs_entails Δ'' (WP fill K (Val $ LitV LitUnit) @ stk; E {{ Φ }}) →
+    envs_entails Δ (WP fill K (store_ty t (PairV (LitV l) v')) @ stk; E {{ Φ }}).
+  Proof.
+    intros Hty.
+    rewrite envs_entails_unseal=> ????.
+    rewrite -wp_bind. eapply bi.wand_apply; first by eapply bi.wand_entails, wp_StoreAt.
+    rewrite into_laterN_env_sound -bi.later_sep envs_simple_replace_sound //; simpl.
+    rewrite right_id. by apply bi.later_mono, bi.sep_mono_r, bi.wand_mono.
+  Qed.
+
+End goose_lang.
+
+Notation "l ↦[ t ] dq v" := (typed_pointsto l dq t v%V)
+                              (at level 20, dq custom dfrac at level 50, t at level 50,
+                               format "l  ↦[ t ] dq  v") : bi_scope.
+
+Tactic Notation "wp_load" :=
+  let solve_pointsto _ :=
+    let l := match goal with |- _ = Some (_, (?l ↦[_]{_} _)%I) => l end in
+    iAssumptionCore || fail "wp_load: cannot find" l "↦[t] ?" in
+  wp_pures;
+  lazymatch goal with
+  | |- envs_entails _ (wp ?s ?E ?e ?Q) =>
+    ( first
+        [reshape_expr e ltac:(fun K e' => eapply (tac_wp_load_ty _ _ _ _ _ K))
+        |fail 1 "wp_load: cannot find 'load_ty' in" e];
+      [tc_solve
+      |solve_pointsto ()
+      |wp_finish] ) ||
+    ( first
+        [reshape_expr e ltac:(fun K e' => eapply (tac_wp_load_ty_persistent _ _ _ _ K))
+        |fail 1 "wp_load: cannot find 'load_ty' in" e];
+      [solve_pointsto ()
+      |wp_finish] )
+  | _ => fail "wp_load: not a 'wp'"
+  end.
+
+Tactic Notation "wp_store" :=
+  let solve_pointsto _ :=
+    let l := match goal with |- _ = Some (_, (?l ↦[_] _)%I) => l end in
+    iAssumptionCore || fail "wp_store: cannot find" l "↦[t] ?" in
+  wp_pures;
+  lazymatch goal with
+  | |- envs_entails _ (wp ?s ?E ?e ?Q) =>
+    first
+      [reshape_expr e ltac:(fun K e' => eapply (tac_wp_store_ty _ _ _ _ _ _ K))
+      |fail 1 "wp_store: cannot find 'store_ty' in" e];
+    [has_go_type
+    |tc_solve
+    |solve_pointsto ()
+    |pm_reflexivity
+    |first [wp_seq|wp_finish]]
+  | _ => fail "wp_store: not a 'wp'"
+  end.
