src/new_goose_lang/lib/slice/slice.v
@@ -1,0 +1,30 @@
+From RecordUpdate Require Import RecordSet.
+From Perennial.Helpers Require Import List Fractional.
+From Perennial.goose_lang Require Import proofmode.
+(* From Perennial.new_goose_lang.lib Require Import persistent_readonly typed_mem. *)
+From Perennial.new_goose_lang.lib Require Export slice.impl.
+From Perennial.goose_lang.lib Require Import control.control.
+
+Set Default Proof Using "Type".
+
+Module slice.
+  Record t :=
+    mk { ptr: loc;
+         sz: u64;
+         cap: u64; }.
+  Global Instance _eta: Settable _ := settable! mk <ptr; sz; cap>.
+  Global Instance _witness: Inhabited _ := populate (mk inhabitant inhabitant inhabitant).
+  Notation extra s := (uint.Z (cap s) - uint.Z (sz s)).
+  Definition nil := mk null (W64 0) (W64 0).
+End slice.
+
+Section goose_lang.
+Context `{ffi_semantics}.
+
+Coercion slice_val (s: slice.t) : val := (#s.(slice.ptr), #s.(slice.sz), #s.(slice.cap)).
+Definition val_slice v : option slice.t :=
+  match v with
+  | (#(LitLoc ptr), #(LitInt sz), #(LitInt cap))%V => Some (slice.mk ptr sz cap)
+  | _ => None
+  end.
+End goose_lang.
